semantics/terminationScript.sml
@@ -134,111 +134,26 @@ Proof
   fs []
 QED
 
-val fix_clock_IMP = Q.prove(
-  `fix_clock s x = (s1,res) ==> s1.clock <= s.clock`,
-  Cases_on `x` \\ fs [fix_clock_def] \\ rw [] \\ fs []);
-
-val (evaluate_def, evaluate_ind) =
-  tprove_no_defn ((evaluateTheory.evaluate_def,evaluateTheory.evaluate_ind),
-  WF_REL_TAC`inv_image ($< LEX $<)
-    (λx. case x of
-         | INL(s,_,es) => (s.clock,exps_size es)
-         | INR(INL (s,_,_,pes,_)) => (s.clock,pes_size pes)
-         | INR(INR (s,_,ds)) => (s.clock,dec1_size ds))` >>
-  rw[size_abbrevs,exp_size_def,dec_clock_def,LESS_OR_EQ,
-     do_if_def,do_log_def,do_eval_res_def,LET_THM] >>
-  imp_res_tac fix_clock_IMP >>
-  simp[SIMP_RULE(srw_ss())[]exps_size_thm,MAP_REVERSE,SUM_REVERSE]);
-
 (* tidy up evalute_def and evaluate_ind *)
 
-Theorem evaluate_clock:
-   (∀(s1:'ffi state) env e r s2. evaluate s1 env e = (s2,r) ⇒ s2.clock ≤ s1.clock) ∧
-   (∀(s1:'ffi state) env v p v' r s2. evaluate_match s1 env v p v' = (s2,r) ⇒ s2.clock ≤ s1.clock) ∧
-   (∀(s1:'ffi state) env ds r s2. evaluate_decs s1 env ds = (s2,r) ⇒ s2.clock ≤ s1.clock)
-Proof
-  ho_match_mp_tac evaluate_ind >> rw[evaluate_def] >>
-  every_case_tac >> fs[] >> rw[] >> rfs[] >>
-  fs[dec_clock_def,fix_clock_def] >> simp[] >>
-  imp_res_tac fix_clock_IMP >> fs[]
-QED
+Theorem evaluate_clock = evaluateTheory.evaluate_clock
 
-Theorem fix_clock_do_eval_res:
-   fix_clock s (do_eval_res vs s) = do_eval_res vs s
-Proof
-  simp [do_eval_res_def]
-  \\ every_case_tac
-  \\ simp [fix_clock_def, state_component_equality]
-QED
+Theorem fix_clock_do_eval_res = evaluateTheory.fix_clock_do_eval_res
 
-Theorem fix_clock_evaluate:
-   fix_clock s1 (evaluate s1 env e) = evaluate s1 env e /\
-   fix_clock s1 (evaluate_decs s1 env ds) = evaluate_decs s1 env ds
-Proof
-  Cases_on `evaluate s1 env e` \\ fs [fix_clock_def]
-  \\ Cases_on `evaluate_decs s1 env ds` \\ fs [fix_clock_def]
-  \\ imp_res_tac evaluate_clock
-  \\ fs [MIN_DEF,state_component_equality]
-QED
-
-val evaluate_def =
-  REWRITE_RULE [fix_clock_evaluate, fix_clock_do_eval_res] evaluate_def
-  |> INST_TYPE[alpha|->``:'ffi``] (* TODO: this is only broken because Lem sucks *);
-
-val evaluate_ind =
-  REWRITE_RULE [fix_clock_evaluate, fix_clock_do_eval_res] evaluate_ind
-  |> INST_TYPE[alpha|->``:'ffi``] (* TODO: this is only broken because Lem sucks *);
+Theorem fix_clock_evaluate = evaluateTheory.fix_clock_evaluate
 
 (* store evaluate_def and evaluate_ind in full and in parts *)
 
-val full_evaluate_def = save_thm("full_evaluate_def",evaluate_def);
-val full_evaluate_ind = save_thm("full_evaluate_ind",evaluate_ind);
+Theorem full_evaluate_def = evaluateTheory.full_evaluate_def
+Theorem full_evaluate_ind = evaluateTheory.full_evaluate_ind
 
-val eval_pat = ``evaluate$evaluate _ _ _``
-val evaluate_conjs =
-  CONJUNCTS full_evaluate_def
-  |> filter (fn th => (th |> SPEC_ALL |> concl |> dest_eq |> fst
-                          |> can (match_term eval_pat)));
+Theorem evaluate_ind = evaluateTheory.evaluate_ind
+Theorem evaluate_match_ind = evaluateTheory.evaluate_match_ind
+Theorem evaluate_decs_ind = evaluateTheory.evaluate_decs_ind
 
-val match_pat = ``evaluate$evaluate_match _ _ _ _ _``
-val evaluate_match_conjs =
-  CONJUNCTS full_evaluate_def
-  |> filter (fn th => (th |> SPEC_ALL |> concl |> dest_eq |> fst
-                          |> can (match_term match_pat)));
-
-val decs_pat = ``evaluate$evaluate_decs _ _ _``
-val evaluate_decs_conjs =
-  CONJUNCTS full_evaluate_def
-  |> filter (fn th => (th |> SPEC_ALL |> concl |> dest_eq |> fst
-                          |> can (match_term decs_pat)));
-
-val evaluate_def = LIST_CONJ (evaluate_conjs @ evaluate_match_conjs);
-
-val evaluate_match_def = LIST_CONJ evaluate_match_conjs;
-
-val evaluate_decs_def = LIST_CONJ evaluate_decs_conjs;
-
-val evaluate_ind = save_thm("evaluate_ind",
-  full_evaluate_ind
-  |> Q.SPECL [`P1`,`P2`,`\v1 v2 v3. T`]
-  |> SIMP_RULE std_ss []
-  |> Q.GENL [`P1`,`P2`]);
-
-val evaluate_match_ind = save_thm("evaluate_match_ind",
-  full_evaluate_ind
-  |> Q.SPECL [`\v1 v2 v3. T`,`P2`,`\v1 v2 v3. T`]
-  |> SIMP_RULE std_ss []
-  |> Q.GEN `P2`);
-
-val evaluate_decs_ind = save_thm("evaluate_decs_ind",
-  full_evaluate_ind
-  |> Q.SPECL [`\v1 v2 v3. T`,`\v1 v2 v3 v4 v5. T`, `P`]
-  |> SIMP_RULE std_ss []
-  |> Q.GEN `P`);
-
-val _ = register "evaluate" evaluate_def evaluate_ind
-val _ = register "evaluate_match" evaluate_match_def evaluate_match_ind
-val _ = register "evaluate_decs" evaluate_decs_def evaluate_decs_ind
+Theorem evaluate_def = evaluateTheory.evaluate_def
+Theorem evaluate_match_def = evaluateTheory.evaluate_match_def
+Theorem evaluate_decs_def = evaluateTheory.evaluate_decs_def
 
 val _ = export_rewrites["evaluate.list_result_def"];
 
